platform/tests/ListBuilder.v
@@ -7,7 +7,7 @@ Definition handlerS := SPEC("sc") reserving 24
 Definition mainS := SPEC reserving 23
   PREonly[_] mallocHeap 0.
 
-Definition m := bimport [[ "malloc"!"malloc" @ [mallocS],
+Definition m := bimport [[ "malloc"!"malloc" @ [mallocS], "malloc"!"free" @ [freeS],
                            "scheduler"!"init" @ [initS], "scheduler"!"exit" @ [exitS],
                            "scheduler"!"spawn" @ [spawnS], "scheduler"!"yield" @ [yieldS] ]]
   bmodule "test" {{
@@ -18,7 +18,7 @@ Definition m := bimport [[ "malloc"!"malloc" @ [mallocS],
       [PREonly[V] Ex ls, sll ls (V "p") * sched (V "sc") * mallocHeap 0]
       While ("i" < 10) {
         "r" <-- Call "malloc"!"malloc"(0, 2)
-        [PREonly[V, R] [| R <> 0 |] * R =?> 2 * Ex ls, sll ls (V "p") * sched (V "sc") * mallocHeap 0];;
+        [PREonly[V, R] [| R <> 0 |] * [| freeable R 2 |] * R =?> 2 * Ex ls, sll ls (V "p") * sched (V "sc") * mallocHeap 0];;
 
         "r" *<- "i";;
         "r" + 4 *<- "p";;
@@ -29,10 +29,24 @@ Definition m := bimport [[ "malloc"!"malloc" @ [mallocS],
         [PREonly[V] Ex ls, sll ls (V "p") * sched (V "sc") * mallocHeap 0]
       };;
 
+      [PREonly[V] Ex ls, sll ls (V "p") * sched (V "sc") * mallocHeap 0]
+      While ("p" <> 0) {
+        "r" <- "p";;
+        "p" <-* "p" + 4;;
+        Call "malloc"!"free"(0, "r", 2)
+        [PREonly[V, R] Ex ls, sll ls (V "p") * sched (V "sc") * mallocHeap 0];;
+
+        Yield
+        [PREonly[V] Ex ls, sll ls (V "p") * sched (V "sc") * mallocHeap 0]
+      };;
+
       Exit
     end with bfunctionNoRet "main"("sc") [mainS]
       "sc" <-- Call "scheduler"!"init"()
       [PREonly[_, R] sched R * mallocHeap 0];;
+
+      Spawn("test"!"handler", 26)
+      [PREonly[V] sched (V "sc") * mallocHeap 0];;
 
       Spawn("test"!"handler", 26)
       [PREonly[V] sched (V "sc") * mallocHeap 0];;
